FraudProof/Winning/Chooser.lean
@@ -1,4 +1,4 @@
-import FraudProof.DataStructures.Value
+-- import FraudProof.DataStructures.Value
 import FraudProof.DataStructures.MTree
 import FraudProof.DataStructures.Hash
 
@@ -17,28 +17,30 @@ open Knowing
 --------------------------------------------------------------------------------
 -- Knowing Chooser.
 --
-def KChooser (gl : Nat) ( hd lt : Hash )
+def KChooser {ℍ : Type}[HashMagma ℍ][BEq ℍ](gl : Nat) ( hd lt : ℍ )
     -- Knowing a path of length |gl| from |hd| to |lt|
     (pathP : Knowing.PathProof gl hd lt)
     -- Cut in position
     ( p : Nat ) ( pLt : p < gl + 1 )
     --
-    ( bot int top : Hash)
+    ( bot int top : ℍ)
     -- One bound is knowledge valid.
     : Chooser.Side
     :=
-    if int = Knowing.inPathProof p pLt pathP -- int = pathNode[p]
-    then if bot = Knowing.inPathProof 0 (by omega) pathP
+    if int == Knowing.inPathProof p pLt pathP -- int = pathNode[p]
+    then if bot == Knowing.inPathProof 0 (by omega) pathP
          then Chooser.Side.Right
          -- If | H : bot = hd ∨ top = lt |, then this is right.
          else Chooser.Side.Left
-    else if top = Knowing.inPathProof gl (by omega) pathP
+    else if top == Knowing.inPathProof gl (by omega) pathP
          then Chooser.Side.Right
          -- If | H : bot = hd ∨ top = lt |, then this is right.
          else Chooser.Side.Left
 
 -- cut here is where is the cut, in Linear games is one, but in Log games is floor (gl/2)
-def KnowingChooser {gl : Nat}{hb ht : Hash}( k : Knowing.PathProof gl hb ht ) (cut : Nat) (cR : cut < gl + 1) : Chooser.Player
+def KnowingChooser {ℍ : Type}{gl : Nat}{hb ht : ℍ}[BEq ℍ][HashMagma ℍ]
+  ( k : Knowing.PathProof gl hb ht ) (cut : Nat) (cR : cut < gl + 1)
+  : Chooser.Player ℍ
   := {
   strategy := KChooser gl hb ht k cut cR
   }
@@ -53,15 +55,15 @@ def KnowingChooser {gl : Nat}{hb ht : Hash}( k : Knowing.PathProof gl hb ht ) (c
 -- -- the root of the tree.
 -- Assuming we are walking trhough a path towards |lt|.
 -- @[simp]
-def LinChooser
+def LinChooser {ℍ : Type}[BEq ℍ]
     -- Knowing elements
-    (hd : Hash) ( nextInPath : Hash)
+    (hd : ℍ) ( nextInPath : ℍ)
     --
-    (head next : Hash )
+    (head next : ℍ )
     : Chooser.Side
     :=
     if head != hd
-    then if next = nextInPath
+    then if next == nextInPath
          then Chooser.Side.Left
          else Chooser.Side.Right
     else -- Head is hd
@@ -69,9 +71,10 @@ def LinChooser
       then Chooser.Side.Left
       else Chooser.Side.Right
 
-def KnowingLinChooserSkl ( len : Nat ) {skl : Fin len -> Unit ⊕ Unit} {hb ht : Hash}
+def KnowingLinChooserSkl {ℍ : Type}[BEq ℍ][HashMagma ℍ]
+   ( len : Nat ) {skl : Fin len -> Unit ⊕ Unit} {hb ht : ℍ}
    ( path : Knowing.PathProofSeq len skl hb ht )
-   : Chooser.LinPlayer len
+   : Chooser.LinPlayer ℍ len
    := {
    strategy := fun p phead pnext =>
    LinChooser
@@ -83,9 +86,10 @@ def KnowingLinChooserSkl ( len : Nat ) {skl : Fin len -> Unit ⊕ Unit} {hb ht :
 }
 -- @[simp]
 def KnowingLinChooser
-   ( len : Nat ) (hb ht : Hash)
+   {ℍ : Type}[BEq ℍ] [HashMagma ℍ]
+   ( len : Nat ) (hb ht : ℍ)
    ( path : Knowing.PathProof len hb ht )
-   : Chooser.LinPlayer len
+   : Chooser.LinPlayer ℍ len
    := {
    strategy := fun p phead pnext =>
    LinChooser
